riscV/Asm.v
@@ -256,7 +256,9 @@ Inductive instruction : Type :=
   (* floating point register move *)
   | Pfmv     (rd: freg) (rs: freg)                  (**r move *)
   | Pfmvxs   (rd: ireg) (rs: freg)                  (**r move FP single to integer register *)
+  | Pfmvsx   (rd: freg) (rs: ireg)                  (**r move integer register to FP single *)
   | Pfmvxd   (rd: ireg) (rs: freg)                  (**r move FP double to integer register *)
+  | Pfmvdx   (rd: freg) (rs: ireg)                  (**r move integer register to FP double *)
 
   (* 32-bit (single-precision) floating point *)
   | Pfls     (rd: freg) (ra: ireg) (ofs: offset)    (**r load float *)
@@ -969,7 +971,9 @@ Definition exec_instr (f: function) (i: instruction) (rs: regset) (m: mem) : out
   | Pfence
 
   | Pfmvxs _ _
+  | Pfmvsx _ _
   | Pfmvxd _ _
+  | Pfmvdx _ _
 
   | Pfmins _ _ _
   | Pfmaxs _ _ _
